rt refine: prove decodeSchedContextInvocation_wf and decode_sc_inv_corres
Signed-off-by: Michael McInerney <Michael.McInerney@data61.csiro.au>

proof/refine/ARM/SchedContextInv_R.thy
@@ -5,7 +5,7 @@
  *)
 
 theory SchedContextInv_R
-imports Ipc_R
+imports Invocations_R Tcb_R
 begin
 
 context begin interpretation Arch . (*FIXME: arch_split*)
@@ -54,30 +54,76 @@ primrec valid_sc_ctrl_inv' :: "sched_control_invocation \<Rightarrow> kernel_sta
 
 primrec sc_inv_rel :: "Invocations_A.sched_context_invocation \<Rightarrow> sched_context_invocation \<Rightarrow> bool"
   where
-  "sc_inv_rel (Invocations_A.InvokeSchedContextConsumed sc bf) sci' =
-   (sci' = InvokeSchedContextConsumed sc bf)"
-| "sc_inv_rel (Invocations_A.InvokeSchedContextBind sc cap) sci' =
-   (\<exists>cap'. cap_relation cap cap' \<and> sci' = InvokeSchedContextBind sc cap')"
-| "sc_inv_rel (Invocations_A.InvokeSchedContextUnbindObject sc cap) sci' =
-   (\<exists>cap'. cap_relation cap cap' \<and> sci' = InvokeSchedContextUnbindObject sc cap')"
-| "sc_inv_rel (Invocations_A.InvokeSchedContextUnbind sc cap) sci' =
-   (sci' = InvokeSchedContextUnbind sc)" \<comment> \<open>FIXME RT: remove cap in abstract InvokeSchedContextUnbind\<close>
-| "sc_inv_rel (Invocations_A.InvokeSchedContextYieldTo sc bf) sci' =
-   (sci' = InvokeSchedContextYieldTo sc bf)"
+  "sc_inv_rel (Invocations_A.InvokeSchedContextConsumed sc_ptr bf) sci' =
+   (sci' = InvokeSchedContextConsumed sc_ptr bf)"
+| "sc_inv_rel (Invocations_A.InvokeSchedContextBind sc_ptr cap) sci' =
+   (\<exists>cap'. cap_relation cap cap' \<and> sci' = InvokeSchedContextBind sc_ptr cap')"
+| "sc_inv_rel (Invocations_A.InvokeSchedContextUnbindObject sc_ptr cap) sci' =
+   (\<exists>cap'. cap_relation cap cap' \<and> sci' = InvokeSchedContextUnbindObject sc_ptr cap')"
+| "sc_inv_rel (Invocations_A.InvokeSchedContextUnbind sc_ptr) sci' =
+   (sci' = InvokeSchedContextUnbind sc_ptr)"
+| "sc_inv_rel (Invocations_A.InvokeSchedContextYieldTo sc_ptr bf) sci' =
+   (sci' = InvokeSchedContextYieldTo sc_ptr bf)"
 
 primrec sc_ctrl_inv_rel ::
   "Invocations_A.sched_control_invocation \<Rightarrow> sched_control_invocation \<Rightarrow> bool" where
-  "sc_ctrl_inv_rel (Invocations_A.InvokeSchedControlConfigure sc budget period refills badge) sci' =
-    (sci' = InvokeSchedControlConfigure sc budget period refills badge)"
+  "sc_ctrl_inv_rel (Invocations_A.InvokeSchedControlConfigure sc_ptr budget period refills badge) sci' =
+    (sci' = InvokeSchedControlConfigure sc_ptr budget period refills badge)"
 
-(* FIXME RT: preconditions can be reduced, this is what is available at the call site: *)
-lemma decodeSchedContextInvocation_wf:
-  "\<lbrace> valid_cap' (SchedContextCap sc n) and invs' and sch_act_simple and ex_nonz_cap_to' sc and
-     (\<lambda>s. \<forall>cap\<in>set excaps. \<forall>r\<in>zobj_refs' cap. ex_nonz_cap_to' r s) and
-     (\<lambda>s. \<forall>x\<in>set excaps. valid_cap' x s) \<rbrace>
-   decodeSchedContextInvocation label sc excaps args
+lemma decodeSchedContext_Bind_wf:
+  "\<lbrace>\<lambda>s. \<exists>n. valid_cap' (SchedContextCap sc_ptr n) s
+        \<and> ex_nonz_cap_to' sc_ptr s
+        \<and> (\<forall>cap\<in>set excaps. \<forall>r\<in>zobj_refs' cap. ex_nonz_cap_to' r s)
+        \<and> (\<forall>x\<in>set excaps. valid_cap' x s)\<rbrace>
+   decodeSchedContext_Bind sc_ptr excaps
    \<lbrace>valid_sc_inv'\<rbrace>, -"
-  sorry
+  apply (clarsimp simp: decodeSchedContext_Bind_def)
+  apply (wpsimp wp: gts_wp' threadGet_wp getNotification_wp
+              simp: scReleased_def scActive_def isBlocked_def refillReady_def)
+  apply (clarsimp simp: valid_cap'_def)
+  apply (drule_tac x="hd excaps" in bspec, fastforce dest: hd_in_set)+
+  apply (fastforce simp: pred_tcb_at'_def obj_at'_def)
+  done
+
+lemma decodeSchedContext_UnbindObject_wf:
+  "\<lbrace>\<lambda>s. \<exists>n. valid_cap' (SchedContextCap sc_ptr n) s
+        \<and> ex_nonz_cap_to' sc_ptr s
+        \<and> (\<forall>cap\<in>set excaps. \<forall>r\<in>zobj_refs' cap. ex_nonz_cap_to' r s)
+        \<and> (\<forall>x\<in>set excaps. valid_cap' x s)\<rbrace>
+   decodeSchedContext_UnbindObject sc_ptr excaps
+   \<lbrace>valid_sc_inv'\<rbrace>, -"
+  apply (clarsimp simp: decodeSchedContext_UnbindObject_def)
+  apply (wpsimp wp: gts_wp' threadGet_wp getNotification_wp
+              simp: scReleased_def scActive_def isBlocked_def refillReady_def)
+  apply (clarsimp simp: valid_cap'_def)
+  apply (drule_tac x="hd excaps" in bspec, fastforce dest: hd_in_set)+
+  apply (fastforce simp: pred_tcb_at'_def obj_at'_def)
+  done
+
+lemma decodeSchedContext_YieldTo_wf:
+  "\<lbrace>\<lambda>s. \<exists>n. valid_cap' (SchedContextCap sc_ptr n) s \<and> ex_nonz_cap_to' sc_ptr s\<rbrace>
+   decodeSchedContext_YieldTo sc_ptr args
+   \<lbrace>valid_sc_inv'\<rbrace>, -"
+  apply (clarsimp simp: decodeSchedContext_YieldTo_def)
+  apply (wpsimp wp: gts_wp' threadGet_wp getNotification_wp getTCB_wp
+              simp: scReleased_def scActive_def isBlocked_def refillReady_def)
+  apply (clarsimp simp: valid_cap'_def)
+  apply (clarsimp simp: pred_tcb_at'_def obj_at'_def projectKOs)
+  done
+
+lemma decodeSchedContextInvocation_wf:
+  "\<lbrace>\<lambda>s. \<exists>n. valid_cap' (SchedContextCap sc_ptr n) s
+        \<and> ex_nonz_cap_to' sc_ptr s
+        \<and> (\<forall>cap\<in>set excaps. \<forall>r\<in>zobj_refs' cap. ex_nonz_cap_to' r s)
+        \<and> (\<forall>x\<in>set excaps. valid_cap' x s)\<rbrace>
+   decodeSchedContextInvocation label sc_ptr excaps args
+   \<lbrace>valid_sc_inv'\<rbrace>, -"
+  apply (simp add: decodeSchedContextInvocation_def)
+  apply (wpsimp wp: decodeSchedContext_Bind_wf
+                    decodeSchedContext_UnbindObject_wf
+                    decodeSchedContext_YieldTo_wf)
+  apply (fastforce dest: valid_SchedContextCap_sc_at')
+  done
 
 (* FIXME RT: preconditions can be reduced, this is what is available at the call site: *)
 lemma decodeSchedControlInvocation_wf:
@@ -88,14 +134,188 @@ lemma decodeSchedControlInvocation_wf:
    \<lbrace>valid_sc_ctrl_inv'\<rbrace>, -"
   sorry
 
+lemma decodeSchedcontext_Bind_corres:
+  "list_all2 cap_relation excaps excaps'
+   \<Longrightarrow> corres (ser \<oplus> sc_inv_rel)
+         (invs and valid_sched and sc_at sc_ptr and (\<lambda>s. \<forall>x\<in>set excaps. s \<turnstile> x))
+         (invs' and (\<lambda>s. \<forall>x\<in>set excaps'. valid_cap' x s))
+         (decode_sched_context_bind sc_ptr excaps)
+         (decodeSchedContext_Bind sc_ptr excaps')"
+  apply (clarsimp simp: decode_sched_context_bind_def decodeSchedContext_Bind_def)
+  apply (cases excaps; clarsimp)
+  apply (rename_tac cap list)
+  apply (cases excaps'; clarsimp)
+  apply (rule corres_splitEE'')
+     apply (corressimp corres: get_sc_corres)
+     apply (fastforce intro: sc_at'_cross_rel[unfolded cross_rel_def, rule_format])
+    apply (rule liftE_validE[THEN iffD2, OF get_sched_context_sp])
+   apply (rule liftE_validE[THEN iffD2, OF get_sc_sp'])
+  apply (rule corres_splitEE_skip; (solves wpsimp)?)
+   apply (corressimp simp: sc_relation_def)
+  apply (case_tac cap; clarsimp)
+   apply (clarsimp simp: bindE_assoc)
+   apply (rule corres_splitEE''[where r'="(=)"]; (solves wpsimp)?)
+    apply (corressimp corres: get_ntfn_corres
+                        simp: get_sk_obj_ref_def ntfn_relation_def valid_cap_def valid_cap'_def
+                          wp: hoare_vcg_all_lift)
+   apply (rule corres_splitEE_skip; (solves wpsimp)?)
+    apply (corressimp corres: get_ntfn_corres
+                        simp: get_sk_obj_ref_def sc_relation_def)
+   apply (clarsimp simp: returnOk_def)
+  apply (clarsimp simp: bindE_assoc get_tcb_obj_ref_def)
+  apply (rule corres_splitEE''[where r'="(=)"])
+     apply (subst corres_liftE_rel_sum)
+     apply (rule corres_guard_imp)
+       apply (rule threadget_corres)
+       apply (clarsimp simp: tcb_relation_def)
+      apply (clarsimp simp: valid_cap_def)
+     apply (clarsimp simp: valid_cap'_def)
+    apply (rule liftE_validE[THEN iffD2, OF thread_get_sp])
+   apply (rule liftE_validE[THEN iffD2, OF threadGet_sp])
+  apply (rule corres_splitEE_skip; (solves \<open>wpsimp simp: valid_cap'_def obj_at'_def\<close>)?)
+   apply (corressimp corres: get_ntfn_corres
+                       simp: get_sk_obj_ref_def sc_relation_def)
+  apply (rule corres_guard_imp)
+    apply (rule corres_split_eqrE)
+       apply (rule corres_splitEE)
+          apply (rule whenE_throwError_corres)
+            apply simp
+           apply simp
+          apply (clarsimp simp: returnOk_def)
+         apply (subst corres_liftE_rel_sum)
+         apply (rule corres_rel_imp)
+          apply (rule gts_isBlocked_corres)
+         apply simp
+        apply wpsimp
+       apply wpsimp
+      apply (rule corres_liftE_rel_sum[THEN iffD2, OF get_sc_released_corres])
+     apply wpsimp
+    apply (wpsimp simp: scReleased_def scActive_def)
+   apply (fastforce simp: obj_at_def is_tcb_def)
+  apply (clarsimp simp: obj_at'_def)
+  done
+
+lemma decodeSchedContext_UnbindObject_corres:
+  "list_all2 cap_relation excaps excaps'
+   \<Longrightarrow> corres (ser \<oplus> sc_inv_rel)
+         (invs and sc_at sc_ptr)
+         invs'
+         (decode_sched_context_unbind_object sc_ptr excaps)
+         (decodeSchedContext_UnbindObject sc_ptr excaps')"
+  apply (clarsimp simp: decode_sched_context_unbind_object_def decodeSchedContext_UnbindObject_def)
+  apply (cases excaps; clarsimp)
+  apply (rename_tac cap list)
+  apply (cases excaps'; clarsimp)
+  apply (case_tac cap; clarsimp)
+   apply (clarsimp simp: bindE_assoc get_sc_obj_ref_def liftE_bind_return_bindE_returnOk)
+   apply (rule corres_splitEE'')
+      apply (corressimp corres: get_sc_corres)
+      apply (fastforce intro: sc_at'_cross_rel[unfolded cross_rel_def, rule_format])
+     apply (rule liftE_validE[THEN iffD2, OF get_sched_context_sp])
+    apply (rule liftE_validE[THEN iffD2, OF get_sc_sp'])
+   apply (corressimp simp: sc_relation_def)
+   apply (clarsimp simp: bindE_assoc get_sc_obj_ref_def liftE_bind_return_bindE_returnOk)
+  apply (rule corres_splitEE'')
+     apply (corressimp corres: get_sc_corres)
+     apply (fastforce intro: sc_at'_cross_rel[unfolded cross_rel_def, rule_format])
+    apply (rule liftE_validE[THEN iffD2, OF get_sched_context_sp])
+   apply (rule liftE_validE[THEN iffD2, OF get_sc_sp'])
+  apply (rule corres_splitEE'')
+     apply (corressimp simp: sc_relation_def)
+    apply (rule whenE_throwError_sp[simplified validE_R_def])+
+  apply (rule corres_splitEE'')
+     apply (corressimp corres: gct_corres)
+    apply (rule liftE_validE[THEN iffD2, OF gets_sp])
+   apply (rule liftE_validE[THEN iffD2, OF getCurThread_sp])
+  apply corressimp
+  done
+
+lemma decodeSchedContext_YieldTo_corres:
+  "corres (ser \<oplus> sc_inv_rel)
+          (invs and sc_at sc_ptr)
+          invs'
+          (decode_sched_context_yield_to sc_ptr args')
+          (decodeSchedContext_YieldTo sc_ptr args')"
+  apply (clarsimp simp: decode_sched_context_yield_to_def decodeSchedContext_YieldTo_def)
+  apply (clarsimp simp: bindE_assoc get_sc_obj_ref_def liftE_bind_return_bindE_returnOk)
+  apply (rule corres_splitEE'')
+     apply (corressimp corres: get_sc_corres)
+     apply (fastforce intro: sc_at'_cross_rel[unfolded cross_rel_def, rule_format])
+    apply (rule liftE_validE[THEN iffD2, OF get_sched_context_sp])
+   apply (rule liftE_validE[THEN iffD2, OF get_sc_sp'])
+  apply (rule corres_splitEE'')
+     apply (corressimp simp: sc_relation_def)
+    apply (rule whenE_throwError_sp[simplified validE_R_def])+
+  apply (rule corres_splitEE'')
+     apply (corressimp corres: gct_corres)
+    apply (rule liftE_validE[THEN iffD2, OF gets_sp])
+   apply (rule liftE_validE[THEN iffD2, OF getCurThread_sp])
+  apply (rule corres_splitEE_skip; (solves wpsimp)?)
+   apply (corressimp simp: sc_relation_def)
+  apply (clarsimp simp: sc_relation_def)
+  apply (rule corres_splitEE''[where r'="(=)"])
+     apply (subst corres_liftE_rel_sum)
+     apply (rule corres_guard_imp)
+       apply (rule threadget_corres)
+       apply (clarsimp simp: tcb_relation_def)
+      apply (fastforce dest: invs_valid_objs valid_objs_ko_at
+                       simp: valid_obj_def valid_sched_context_def)
+     apply (fastforce dest: sc_ko_at_valid_objs_valid_sc'
+                      simp: valid_sched_context'_def)
+    apply (rule liftE_validE[THEN iffD2, OF thread_get_sp])
+   apply (rule liftE_validE[THEN iffD2, OF threadGet_sp])
+  apply (rule corres_splitEE''[where r'="(=)"])
+     apply (subst corres_liftE_rel_sum)
+     apply (rule corres_guard_imp)
+       apply (rule threadget_corres)
+       apply (clarsimp simp: tcb_relation_def)
+      apply fastforce
+     apply fastforce
+    apply (rule liftE_validE[THEN iffD2, OF thread_get_sp])
+   apply (rule liftE_validE[THEN iffD2, OF threadGet_sp])
+  apply (rule corres_splitEE_skip; corressimp)
+  apply (rule corres_splitEE''[where r'="(=)"])
+     apply (subst corres_liftE_rel_sum)
+     apply (rule corres_guard_imp)
+       apply (rule threadget_corres)
+       apply (clarsimp simp: tcb_relation_def)
+      apply fastforce
+     apply fastforce
+    apply (rule liftE_validE[THEN iffD2, OF thread_get_sp])
+   apply (rule liftE_validE[THEN iffD2, OF threadGet_sp])
+  apply (rule corres_splitEE_skip; corressimp)
+  apply (clarsimp simp: obj_at'_def)
+  done
+
 lemma decode_sc_inv_corres:
   "list_all2 cap_relation excaps excaps' \<Longrightarrow>
    corres (ser \<oplus> sc_inv_rel)
-          (invs and valid_sched and sc_at sc and (\<lambda>s. \<forall>x\<in>set excaps. s \<turnstile> x))
+          (invs and valid_sched and sc_at sc_ptr and (\<lambda>s. \<forall>x\<in>set excaps. s \<turnstile> x))
           (invs' and (\<lambda>s. \<forall>x\<in>set excaps'. valid_cap' x s))
-          (decode_sched_context_invocation (mi_label mi) sc excaps args')
-          (decodeSchedContextInvocation (mi_label mi) sc excaps' args')"
-  sorry
+          (decode_sched_context_invocation (mi_label mi) sc_ptr excaps args')
+          (decodeSchedContextInvocation (mi_label mi) sc_ptr excaps' args')"
+  apply (clarsimp simp: decode_sched_context_invocation_def decodeSchedContextInvocation_def
+             split del: if_split)
+  apply (cases "gen_invocation_type (mi_label mi)"
+         ; clarsimp split: gen_invocation_labels.split list.splits
+                split del: if_split)
+      apply (clarsimp simp: returnOk_def)
+     apply (corressimp corres: decodeSchedcontext_Bind_corres)
+    defer
+    apply (corressimp corres: decodeSchedContext_UnbindObject_corres)
+   apply (corressimp corres: decodeSchedContext_YieldTo_corres)
+  apply (rule corres_splitEE'')
+     apply (corressimp corres: get_sc_corres)
+     apply (fastforce intro: sc_at'_cross_rel[unfolded cross_rel_def, rule_format])
+    apply (rule liftE_validE[THEN iffD2, OF get_sched_context_sp])
+   apply (rule liftE_validE[THEN iffD2, OF get_sc_sp'])
+  apply (rule corres_splitEE'')
+     apply (corressimp corres: gct_corres)
+    apply (rule liftE_validE[THEN iffD2, OF gets_sp])
+   apply (rule liftE_validE[THEN iffD2, OF getCurThread_sp])
+  apply (rule corres_splitEE_skip; corressimp)
+  apply (clarsimp simp: sc_relation_def)
+  done
 
 lemma decode_sc_ctrl_inv_corres:
   "list_all2 cap_relation excaps excaps' \<Longrightarrow>
